src/program_proof/rsm/distx/invariance/learn_abort.v
@@ -43,9 +43,9 @@ Section inv.
     map_Forall (λ _ t, t.2 = ts) tpls ->
     txnres_abt γ ts -∗
     ([∗ map] key ↦ tpl ∈ tpls, key_inv_no_repl_tsprep γ key tpl.1 tpl.2) -∗
-    txn_inv γ -∗
+    txnsys_inv γ -∗
     ([∗ map] key ↦ tpl ∈ tpls, key_inv_prepared_no_repl_tsprep γ key tpl.1 ts) ∗
-    txn_inv γ.
+    txnsys_inv γ.
   Proof.
     iIntros (Hts) "#Habt Htpls Htxn".
     iApply (big_sepM_impl_res with "Htpls Htxn").
@@ -114,10 +114,10 @@ Section inv.
 
   Lemma group_inv_learn_abort γ gid log cpool ts :
     cpool_subsume_log cpool (log ++ [CmdAbt ts]) ->
-    txn_inv γ -∗
+    txnsys_inv γ -∗
     ([∗ set] key ∈ keys_all, key_inv γ key) -∗
     group_inv_no_log_with_cpool γ gid log cpool ==∗
-    txn_inv γ ∗
+    txnsys_inv γ ∗
     ([∗ set] key ∈ keys_all, key_inv γ key) ∗
     group_inv_no_log_with_cpool γ gid (log ++ [CmdAbt ts]) cpool.
   Proof.
